backend/Mach.v
@@ -396,9 +396,10 @@ Inductive step: state -> trace -> state -> Prop :=
       step (State s fb (Vptr stk soff) (Mreturn :: c) rs m)
         E0 (Returnstate s rs m')
   | exec_function_internal:
-      forall s fb rs m f m1 m2 m3 stk rs',
+      forall s fb rs m f m1 m2 m3 stk rs'
+      (STK: stk = fresh_block (support m)),
       Genv.find_funct_ptr ge fb = Some (Internal f) ->
-      Mem.alloc m 0 f.(fn_stacksize) = (m1, stk) ->
+      Mem.alloc m 0 f.(fn_stacksize) stk = Some m1 ->
       let sp := Vptr stk Ptrofs.zero in
       store_stack m1 sp Tptr f.(fn_link_ofs) (parent_sp s) = Some m2 ->
       store_stack m2 sp Tptr f.(fn_retaddr_ofs) (parent_ra s) = Some m3 ->
